Add task constructors, theory hashcons

extract/TaskExn.ml
@@ -1,0 +1,3 @@
+exception LemmaFound
+exception GoalFound
+exception GoalNotFound
