src/core/TaskFuncs.v
@@ -1,0 +1,99 @@
+Require Export TaskDefs.
+Import MonadNotations.
+(* Constructors with Checks*)
+
+Definition LemmaFound : errtype :=
+  mk_errtype "LemmaFound" tt.
+Definition GoalFound : errtype :=
+  mk_errtype "GoalFound" tt.
+Definition GoalNotFound : errtype :=
+  mk_errtype "GoalNotFound" tt.
+
+Definition find_goal (t: task) : option (prsymbol * term_c) :=
+  option_bind t (fun t =>
+  match td_node_of t.(task_decl) with
+  | Decl d =>
+    match d.(d_node) with
+    | Dprop x =>
+      let '(k, p, f) := of_tup3 x in
+      match k with
+      | Pgoal => Some (p, f)
+      | _ => None
+      end
+    | _ => None
+    end
+  | _ => None
+  end).
+
+Definition task_goal (t: task) : errorM prsymbol :=
+  match find_goal t with
+  | Some (pr, _) => err_ret pr
+  | _ => throw GoalNotFound
+  end.
+
+Definition task_goal_fmla (t: task) : errorM term_c :=
+  match find_goal t with
+  | Some(_, f) => err_ret f
+  | _ => throw GoalNotFound
+  end.
+
+Definition task_separate_goal (t: task) : errorM (tdecl_c * task) :=
+ match t with
+ | Some t =>
+  match td_node_of t.(task_decl) with
+  | Decl d =>
+    match d.(d_node) with
+    | Dprop x =>
+      let '(k, p, f) := of_tup3 x in
+      match k with
+      | Pgoal => err_ret (t.(task_decl), t.(task_prev))
+      | _ => throw GoalNotFound
+      end
+    | _ => throw GoalNotFound
+    end
+  | _ => throw GoalNotFound
+  end
+  | _ => throw GoalNotFound
+ end.
+
+Definition check_task (t: task) : errorM task := 
+  match find_goal t with
+  | Some _  => throw GoalFound
+  | None    => err_ret t
+  end.
+
+Definition check_decl (d: decl) : errorM decl :=
+  match d.(d_node) with
+  | Dprop x =>
+    let '(k, _, _) := of_tup3 x in
+    match k with
+    | Plemma => throw LemmaFound
+    | _ => err_ret d
+    end
+  | _ => err_ret d
+  end.
+
+Local Open Scope errst_scope.
+(*TODO: how to avoid all of the lifts?*)
+Definition new_decl1 (t: task) (d : decl) (td: tdecl_c) : 
+  errState (hashcons_ty tdecl_c * hashcons_ty task_hd) (known_res task) :=
+  d1 <- errst_lift2 (check_decl d);;
+  o <- errst_lift2 (known_add_decl_informative (task_known1 t) d1);;
+  match o with
+  | Known i => errst_ret (Known _ i)
+  | Normal (d1, kn) =>
+  td1 <- errst_lift1 (st_lift1 (create_decl d1)) ;;
+  _ <- errst_lift2 (check_task t);;
+  h <- errst_lift1 (st_lift2 (mk_task td1 t kn (task_clone1 t) (task_meta1 t)));;
+  errst_ret (Normal _ h)
+  end.
+
+(*Why we needed this known_res stuff*)
+Definition new_decl (t: task) (d: decl) (td: tdecl_c) : errState (hashcons_ty tdecl_c * hashcons_ty task_hd) task :=
+  o <- new_decl1 t d td ;;
+  match o with
+  | Known i => errst_ret t
+  | Normal n => errst_ret n
+  end.
+
+(*Skip [new_clone], [new_meta]*)
